Skeleton for axiomatic-to-promising proof

src/AtoP.v
@@ -14,8 +14,9 @@ Require Import HahnRelationsBasic.
 Require Import Order.
 Require Import Time.
 Require Import Lang.
-Require Import Axiomatic.
+Require Import Memory.
 Require Import Promising.
+Require Import Axiomatic.
 
 Set Implicit Arguments.
 
@@ -28,27 +29,102 @@ Lemma linearize A
     <<PERM: Permutation l l'>> /\
     <<REL: forall i j x y
              (X: List.nth_error l' i = Some x)
-             (X: List.nth_error l' j = Some y),
-        ~ rel y x>>.
+             (X: List.nth_error l' j = Some y)
+             (REL: rel x y),
+        i < j>>.
 Proof.
-  (* TODO
-     - Pick an element x.
-     - Split the list: BEFORE:={y | rtc rel y x} and the others AFTER
-     - Linearize BEFORE, place x, and then linearize AFTER.
-   *)
+Admitted.
+
+Inductive sim_label (tid:Id.t): forall (label:Label.t) (msg:Msg.t), Prop :=
+| sim_label_intro
+    ex ord loc val:
+    sim_label tid (Label.write ex ord loc val) (Msg.mk loc val tid)
+.
+Hint Constructors sim_label.
+
+(* TODO: move *)
+Fixpoint filter_map A B (f: A -> option B) (l: list A): list B :=
+  match l with
+  | [] => []
+  | a::l =>
+    match f a with
+    | None => filter_map f l
+    | Some b => b :: filter_map f l
+    end
+  end.
+
+Definition construct_mem
+           (ex:Execution.t)
+           (eids:list eidT):
+  Memory.t :=
+  filter_map
+    (fun eid =>
+       match Execution.label eid ex with
+       | Some (Label.write ex ord loc val) => Some (Msg.mk loc val eid.(fst))
+       | _ => None
+       end)
+    eids.
+
+Inductive sim (ex:Execution.t) (m: Machine.t): Prop :=
+| sim_intro
+    eids
+    (EIDS: Permutation eids (Execution.eids ex))
+    (OB: forall i j x y
+           (X: List.nth_error eids i = Some x)
+           (X: List.nth_error eids j = Some y)
+           (OB: ex.(Execution.ob) x y),
+        i < j)
+    (MEM: m.(Machine.mem) = construct_mem ex eids)
+.
+Hint Constructors sim.
+
+Lemma promise_mem
+      p mem
+      (MEM: forall msg (MSG: List.In msg mem), IdMap.find msg.(Msg.tid) p <> None):
+  exists m,
+    <<STEP: rtc Machine.step0 (Machine.init p) m>> /\
+    <<TPOOL: m.(Machine.tpool) = (Machine.init p).(Machine.tpool)>> /\ (* TODO: Local.promises.. *)
+    <<MEM: m.(Machine.mem) = mem>>.
+Proof.
+  revert MEM. induction mem using List.rev_ind; i.
+  { esplits; eauto. }
+  exploit IHmem; eauto.
+  { i. apply MEM. apply List.in_app_iff. intuition. }
+  i. des. subst. destruct x.
+  hexploit MEM.
+  { apply List.in_app_iff. right. left. eauto. }
+  match goal with
+  | [|- context[?f]] => destruct f eqn:FIND
+  end; ss.
+  intro X. clear X.
+  eexists (Machine.mk _ _). esplits.
+  - etrans; [eauto|]. econs 2; [|refl].
+    econs.
+    + rewrite TPOOL, IdMap.map_spec, FIND. ss.
+    + econs 2; ss. econs; eauto. ss.
+    + ss.
+  - admit. (* Local.promises is updated *)
+  - ss.
 Admitted.
 
 Lemma axiomatic_to_promising
       p ex
       (AXIOMATIC: is_valid p ex):
-  False.
+  exists m,
+    <<STEP: rtc Machine.step (Machine.init p) m>> /\
+    <<SIM: sim ex m>>.
 Proof.
-  
+  (* Linearize events and construct memory. *)
+  exploit (linearize (Execution.eids ex)).
+  { inv AXIOMATIC. apply EXTERNAL. }
+  i. des. rename l' into eids.
+  remember (construct_mem ex eids) as mem eqn:MEM.
 
+  (* Construct promise steps. *)
+  exploit (promise_mem p mem); eauto.
+  { i. subst. admit. }
+  i. des.
 
-
-  (* TODO
-
-     - Give an order on all writes using `ob`.
-   *)
+  (* TODO: execute each thread. *)
+  admit.
 Admitted.
